Worked on context_conversion for red

extraction/theories/EArities.v
@@ -46,9 +46,132 @@ Admitted.                       (* constructors have a type *)
   
 (* Admitted. (* projections have a type *) *)
 
-Lemma context_conversion_red (Σ : global_env_ext) Γ Γ' s t : wf Σ ->
-  PCUICSR.conv_context Σ Γ Γ' -> red Σ Γ s t -> red Σ Γ' s t.
-Admitted.
+Inductive conv_decls Σ Γ (Γ' : context) : forall (x y : context_decl), Type :=
+| conv_vass : forall (na na' : name) (T T' : term),
+                isWfArity_or_Type Σ Γ' T' ->
+                Σ;;; Γ |- T = T' -> conv_decls Σ Γ Γ' (vass na T) (vass na' T')
+| conv_vdef_type : forall (na : name) (b T  : term),
+    isWfArity_or_Type Σ Γ' T ->
+    conv_decls Σ Γ Γ' (vdef na b T) (vdef na b T).
+
+Lemma conv_context_refl Σ Γ : wf Σ -> wf_local Σ Γ -> context_relation conv_decls Σ Γ Γ.
+Proof.
+  induction Γ; try econstructor. 
+  intros wfΣ wfΓ; depelim wfΓ; econstructor; eauto;
+  constructor; auto.
+  - right. eassumption.
+  - apply conv_refl.
+  - right. eassumption.
+Qed.
+
+Lemma context_conversion_red1 Σ Γ Γ' s t T : wf Σ -> Σ ;;; Γ' |- t : T ->
+   context_relation conv_decls Σ Γ Γ' -> red1 Σ Γ s t -> red Σ Γ' s t.
+Proof.
+  intros HΣ HT X X0. induction X0 using red1_ind_all in Γ', HΣ, HT, X, T |- *; eauto.
+  Hint Constructors red red1.
+  all:eauto.
+  - econstructor. econstructor. econstructor.
+    rewrite <- H. 
+    induction X in i |- *; destruct i; eauto.
+    now inv p. 
+  - eapply inversion_Lambda in HT as (? & ? & ? & ? & ?).
+    eapply PCUICReduction.red_abs. eapply IHX0; eauto.  eauto.
+  - eapply inversion_Lambda in HT as (? & ? & ? & ? & ?).
+    eapply PCUICReduction.red_abs. eauto. eapply IHX0. eauto. 
+    eauto. econstructor. eauto. econstructor. 2:eapply conv_refl. 
+    right. econstructor. eauto. 
+  - eapply inversion_LetIn in HT as (? & ? & ? & ? & ?).
+    eapply PCUICReduction.red_letin. eapply IHX0; eauto. 
+    all:eauto. 
+  - eapply inversion_LetIn in HT as (? & ? & ? & ? & ?).
+    eapply PCUICReduction.red_letin; eauto. 
+  - eapply inversion_LetIn in HT as (? & ? & ? & ? & ? & ?).
+    eapply PCUICReduction.red_letin; eauto. eapply IHX0; eauto. 
+    econstructor. eauto. econstructor. right; eexists; eauto.
+  - destruct ind. eapply inversion_Case in HT as (? & ? & ? & ? & ? & ? & ? & ? & ? & ? & ? & ? & ? & ? & ? & ? & ? & ?). subst.
+    eapply PCUICReduction.reds_case; eauto. clear.
+    eapply PCUICCumulativity.All_All2_refl. induction brs; eauto.
+  -  destruct ind. eapply inversion_Case in HT as (? & ? & ? & ? & ? & ? & ? & ? & ? & ? & ? & ? & ? & ? & ? & ? & ? & ?). subst.
+     eapply PCUICReduction.reds_case; eauto. clear.
+    eapply PCUICCumulativity.All_All2_refl. induction brs; eauto.
+  - destruct ind. eapply inversion_Case in HT as (? & ? & ? & ? & ? & ? & ? & ? & ? & ? & ? & ? & ? & ? & ? & ? & ? & ?). subst.
+    eapply PCUICReduction.reds_case; eauto. 
+    clear - HΣ X0 a t X.
+    induction X0 in x7, a |- *.
+    + inv a. econstructor. destruct p0. destruct p0.
+      split; eauto. eapply r0; eauto. firstorder. 
+      eapply PCUICCumulativity.All_All2_refl. 
+      induction X1; eauto. 
+    + inv a. econstructor.  repeat econstructor.
+      eapply IHX0. eauto.
+  - eapply inversion_Proj in HT as (? & ? & ? & ? & ? & ? & ? & ? & ?).
+    eapply PCUICReduction.red_proj_c. eauto.
+  - eapply inversion_App in HT as (? & ? & ? & ? & ? & ?).
+    eapply PCUICReduction.red_app; eauto.
+  - eapply inversion_App in HT as (? & ? & ? & ? & ? & ?).
+    eapply PCUICReduction.red_app; eauto.
+  - eapply inversion_Prod in HT as (? & ? & ? & ? & ?).
+    eapply PCUICReduction.red_prod; eauto.
+  - eapply inversion_Prod in HT as (? & ? & ? & ? & ?).
+    eapply PCUICReduction.red_prod; eauto. eapply IHX0. eauto. eauto. 
+    econstructor. 
+    eauto. econstructor. right. econstructor. eauto. eapply conv_refl.
+  - now eapply inversion_Evar in HT.
+  - eapply inversion_Fix in HT as ( ? & ? & ? & ? & ?).
+    eapply PCUICReduction.red_fix_congr; eauto.
+    generalize (fix_context mfix0). intros.
+    induction X0; eauto. 
+    destruct p. inv a0. destruct p.
+    econstructor; eauto. split. inv e0. eapply r0; eauto. admit.
+    inv e0. econstructor. clear.
+    eapply PCUICCumulativity.All_All2_refl. induction tl; eauto.
+    econstructor. eauto. admit.
+  - eapply inversion_Fix in HT as ( ? & ? & ? & ? & ?).
+    eapply PCUICReduction.red_fix_congr; eauto. 
+    remember (fix_context mfix0). intros. (* clear Heqc. *)
+    (* induction X1 in  |- *; eauto.  *)
+    (* destruct p. destruct p. *)
+    (* econstructor; eauto. split. inv e. econstructor. eapply r0.  *)
+    (* inv e. *)
+    (* * clear - X0. induction c. eassumption. cbn. destruct a.  *)
+    (*   destruct decl_body. econstructor. eassumption. econstructor. *)
+    (*   econstructor.  eauto. econstructor. econstructor. *)
+    (* * clear.  *)
+    (*   eapply PCUICCumulativity.All_All2_refl. induction tl; eauto. *)
+  (* - eapply PCUICReduction.red_cofix_congr; eauto.  *)
+  (*   generalize (fix_context mfix0). intros. *)
+  (*   induction X1; eauto.  *)
+  (*   destruct p. destruct p. *)
+  (*   econstructor; eauto. split. eapply r0. eauto. *)
+  (*   inv e. econstructor. *)
+  (*   clear. *)
+  (*   eapply PCUICCumulativity.All_All2_refl. induction tl; eauto. *)
+  (* - eapply PCUICReduction.red_cofix_congr; eauto. *)
+  (*   remember (fix_context mfix0). intros. clear Heqc. *)
+  (*   induction X1 in  |- *; eauto.  *)
+  (*   destruct p. destruct p. *)
+  (*   econstructor; eauto. split. inv e. econstructor. eapply r0.  *)
+  (*   inv e. *)
+  (*   * clear - X0. induction c. eassumption. cbn. destruct a.  *)
+  (*     destruct decl_body. econstructor. eassumption. econstructor. *)
+  (*     econstructor.  eauto. econstructor. econstructor. *)
+  (*   * clear.  *)
+  (*     eapply PCUICCumulativity.All_All2_refl. induction tl; eauto. *)
+Admitted. 
+
+Lemma context_conversion_red Σ Γ Γ' s t T : wf Σ -> Σ ;;; Γ |- s : T ->
+  context_relation conv_decls Σ Γ Γ' -> red Σ Γ s t -> red Σ Γ' s t.
+Proof.
+  intros. induction X2; eauto. 
+  etransitivity. eapply IHX2.
+  eapply context_conversion_red1; eauto.
+  eapply context_conversion; sq; eauto. 
+  eapply RedFlags.default. 
+  eapply subject_reduction. eauto. eauto. eauto. 
+  clear - X1. induction X1; try inv p; econstructor; eauto.
+  econstructor; eauto.
+  econstructor. eauto. eapply conv_refl.
+Qed.
 
 Lemma invert_cumul_arity_r (Σ : global_env_ext) (Γ : context) (C : term) T :
   wf Σ -> wf_local Σ Γ ->
@@ -66,11 +189,11 @@ Proof.
     etransitivity. eauto.
     eapply PCUICReduction.red_prod_r.
 
-    eapply context_conversion_red. eauto. 2:eauto.
-    econstructor. eapply PCUICSR.conv_ctx_refl; eauto.
+  (*   eapply context_conversion_red. eauto. 2:eauto. *)
+  (*   + econstructor. clear; induction Γ. econstructor. destruct a, decl_body. econstructor. eauto. econstructor. econstructor. eauto. econstructor. eauto. econstructor. *)
 
-    econstructor. 2:eauto. 2:econstructor; eauto. 2:cbn. admit. admit.
-  -   admit.
+  (*   econstructor. 2:eauto. 2:econstructor; eauto. 2:cbn. admit. admit. *)
+  (* -   admit. *)
 Admitted.                       (* invert_cumul_arity_r *)
 
 Lemma invert_cumul_arity_l (Σ : global_env_ext) (Γ : context) (C : term) T :
@@ -89,34 +212,14 @@ Proof.
     etransitivity. eauto.
     eapply PCUICReduction.red_prod_r.
 
-    eapply context_conversion_red. eauto. 2:eauto.
-    econstructor. eapply conv_ctx_refl; eauto.
+  (*   eapply context_conversion_red. eauto. 2:eauto. *)
+  (*   econstructor. eapply conv_context_refl; eauto.  *)
 
-    econstructor. 2:eauto. 2:econstructor; eauto. 2:cbn. admit. admit.
-  - eapply invert_cumul_letin_l in X; eauto.
+  (*   econstructor. 2:eauto. 2:econstructor; eauto. 2:cbn. admit. admit. *)
+  (* - eapply invert_cumul_letin_l in X; eauto. *)
 Admitted.                       (* invert_cumul_arity_l *)
 
-Lemma isWfArity_prod_inv:
-  forall (Σ : global_env_ext) (Γ : context) (T : term) (x : name) (x0 x1 : term),
-    isWfArity typing Σ Γ (tProd x x0 x1) -> (∑ s : universe, Σ;;; Γ |- x0 : tSort s) ×   isWfArity typing Σ (Γ,, vass x x0) x1
-.
-Proof.
-  
-           
-           (* destruct X as (? & ? & ? & ?). cbn in e. *)
-           (* change (Γ ,, vass x x0) with (Γ ,,, [vass x x0]). unfold ",," in e. *)
-           (* revert e. *)
-           (* generalize ([vass x x0]). intros. *)
-           (* induction x1 in l, e |- *; cbn in *; try now inv e. *)
-           (* ++ inv e. repeat econstructor. cbn. eauto. *)
-           (* ++ eapply IHx1_2 in e as (? & ? & ? & ?). *)
-           (*    repeat econstructor. cbn. admit. admit. (* destArity stuff *) *)
-           (* ++ eapply IHx1_3 in e as (? & ? & ? & ?). *)
-           (*    repeat econstructor. cbn. admit. admit. (* destArity stuff *) *)
-  
-Admitted.                       (* inversion for isWfarity on products *)
-
-Lemma arity_type_inv (Σ : global_env_ext) Γ t T1 T2 : wf Σ -> wf_local Σ Γ ->
+Lemma arity_type_inv Σ Γ t T1 T2 : wf Σ -> wf_local Σ Γ ->
   Σ ;;; Γ |- t : T1 -> isArity T1 -> Σ ;;; Γ |- t : T2 -> Is_conv_to_Arity Σ Γ T2.
 Proof.
   intros wfΣ wfΓ. intros. eapply principal_typing in X as (? & ? & ? & ?). 2:eauto. 2:exact X0.
